{"cells":[{"metadata":{},"cell_type":"markdown","source":"# Problem 1\n\nGiven the following $Y(s)$ that represents the unit step response of a dynamical system:\n\n$$Y(s)=\\frac{s+12}{s(s+3)}=\\frac{c_1}{s}+\\frac{c_2}{s+3}$$"},{"metadata":{},"cell_type":"markdown","source":"## a) \n\nUse partial fraction expansion (*delbrøksoppløsning*) and find the coefficients $c_1$ and $c_2$;"},{"metadata":{"trusted":false},"cell_type":"code","source":"import sympy as sym\ns, c_1, c_2 = sym.symbols('s,c_1,c_2')\n\nY = sym.Eq((s+12)/(s*(s+3)),c_1/s + c_2/(s+3))\ndisplay(Y)\n\nsym.solve(Y,(c_1,c_2))","execution_count":1,"outputs":[{"output_type":"display_data","data":{"text/plain":"Eq((s + 12)/(s*(s + 3)), c_1/s + c_2/(s + 3))","text/latex":"$\\displaystyle \\frac{s + 12}{s \\left(s + 3\\right)} = \\frac{c_{1}}{s} + \\frac{c_{2}}{s + 3}$"},"metadata":{}},{"output_type":"execute_result","execution_count":1,"data":{"text/plain":"{c_1: 4, c_2: -3}"},"metadata":{}}]},{"metadata":{},"cell_type":"markdown","source":"## b)\n\nUse the inverse Laplace transform from the Laplace-table and determine $y(t)$;"},{"metadata":{},"cell_type":"markdown","source":"utkast av tabellen:\n\n| $s$-plane       | $t$-plane  |\n| --------------- | ---------- |\n| $\\frac{k}{s}$   | $k$        |\n| $\\frac{k}{a+s}$ | $ke^{-at}$ |\n\nsince the equation is:\n$$\\frac{4}{s}-\\frac{3}{s+3}$$\n\nand since Laplace is a linear operator we can split the terms\n\n$\\frac{4}{s}$ and $-\\frac{3}{s+3}$\n\n$$\\frac{4}{s} = \\mathscr{L}\\{4\\}$$\n\n$$-\\frac{3}{s+3} = \\mathscr{L}\\{-3e^{-3t}\\}$$\n\nand here is a script for verification:"},{"metadata":{"trusted":false},"cell_type":"code","source":"import sympy as sym\ns,t = sym.symbols('s,t')\nY = sym.apart((s+12)/(s*(s+3)))\ndisplay(Y)\n\n\ny = sym.simplify(\n        sym.inverse_laplace_transform(Y,s,t)\n        /\n        sym.Heaviside(t))\n\ndisplay(y)","execution_count":2,"outputs":[{"output_type":"display_data","data":{"text/plain":"-3/(s + 3) + 4/s","text/latex":"$\\displaystyle - \\frac{3}{s + 3} + \\frac{4}{s}$"},"metadata":{}},{"output_type":"display_data","data":{"text/plain":"4 - 3*exp(-3*t)","text/latex":"$\\displaystyle 4 - 3 e^{- 3 t}$"},"metadata":{}}]},{"metadata":{},"cell_type":"markdown","source":"## c)\n\nWhat is the final value of the output $y(\\infty)$ (when $t \\rightarrow \\infty$)?"},{"metadata":{"trusted":false},"cell_type":"code","source":"import sympy as sym\ns,t= sym.symbols(\"s,t\")\n\nY = sym.apart((s+12)/(s*(s+3)))\n\ny = sym.simplify(\n        sym.inverse_laplace_transform(Y,s,t)\n        /\n        sym.Heaviside(t))\ndisplay(y)\n\nz = sym.simplify(\n        sym.inverse_laplace_transform(Y,s,t))\n\ndisplay(z)\ndisplay(y.subs(t,sym.oo))\ndisplay(z.subs(t,sym.oo))","execution_count":3,"outputs":[{"output_type":"display_data","data":{"text/plain":"4 - 3*exp(-3*t)","text/latex":"$\\displaystyle 4 - 3 e^{- 3 t}$"},"metadata":{}},{"output_type":"display_data","data":{"text/plain":"(4*exp(3*t) - 3)*exp(-3*t)*Heaviside(t)","text/latex":"$\\displaystyle \\left(4 e^{3 t} - 3\\right) e^{- 3 t} \\theta\\left(t\\right)$"},"metadata":{}},{"output_type":"display_data","data":{"text/plain":"4","text/latex":"$\\displaystyle 4$"},"metadata":{}},{"output_type":"display_data","data":{"text/plain":"nan","text/latex":"$\\displaystyle \\text{NaN}$"},"metadata":{}}]},{"metadata":{},"cell_type":"markdown","source":"# Problem 2\n\nA dynamic system having the output $h(t)$, the input $g(t)$ and all the initial values negligible is described:\n$$\\frac{d^4h(t)}{{dt}^4}+3\\frac{d^3h(t)}{{dt}^3}+7\\frac{d^2h(t)}{{dt}^2}+4h(t)=2\\frac{d^3g(t)}{{dt}^3}+11\\frac{d^2g(t)}{{dt}^2}+4\\frac{dg(t)}{dt}+12g(t)$$"},{"metadata":{},"cell_type":"markdown","source":"## a)\n\nFind the transfer function of the system $W(s)=\\frac{H(s)}{G(s)}$"},{"metadata":{},"cell_type":"markdown","source":"i want to use the formula:\n\n$$\\frac{d^{n+1}f(t)}{{dt}^{n+1}} = s^{n+1}F(s)-\\sum^n_{i=0}{s^{n-i}\\frac{d^if(t)}{{dt}^i}}$$\n\nand since the task is telling me the initial values is negligible i can crude the the formula to:\n\n$$\\frac{d^{n+1}f(t)}{{dt}^{n+1}} = s^{n+1}F(s)$$\n\nletting me write the equation\n\n$$\\frac{d^4h(t)}{{dt}^4}+3\\frac{d^3h(t)}{{dt}^3}+7\\frac{d^2h(t)}{{dt}^2}+4h(t)=2\\frac{d^3g(t)}{{dt}^3}+11\\frac{d^2g(t)}{{dt}^2}+4\\frac{dg(t)}{dt}+12g(t)$$\n\nas:\n\n$$s^4H(s)+3s^3H(s)+7s^2H(s)+4H(s)=2s^3G(s)+11s^2G(s)+4sG(s)+12G(s)$$\n\nfactorise it as:\n\n$$H(s)(s^4+3s^3+7s^2+4)=G(s)(2s^3+11s^2+4s+12)$$\n\nand to get the form:\n\n$$W(s)=\\frac{H(s)}{G(s)}$$\n\ni can factorise the equation:\n\n$$\\frac{H(s)(s^4+3s^3+7s^2+4)}{G(s)(s^4+3s^3+7s^2+4)}=\\frac{G(s)(2s^3+11s^2+4s+12)}{G(s)(s^4+3s^3+7s^2+4)}$$\n\n$$\\frac{H(s)}{G(s)}=\\frac{(2s^3+11s^2+4s+12)}{(s^4+3s^3+7s^2+4)}$$\n\n$$W(s)=\\frac{H(s)}{G(s)}$$\n\n$$W(s)=\\frac{H(s)}{G(s)}=\\frac{(2s^3+11s^2+4s+12)}{(s^4+3s^3+7s^2+4)}$$"},{"metadata":{},"cell_type":"markdown","source":"## b)\n\nwhat is the final value of the output $h(\\infty)$ when the input is a step with magnitude 150?"},{"metadata":{},"cell_type":"markdown","source":"This is a step response of $150$, meaning $G(s)=\\frac{150}{s}$\n\nusing this the transferfunction of the system:\n\n$$\\frac{H(s)}{G(s)}=\\frac{(2s^3+11s^2+4s+12)}{(s^4+3s^3+7s^2+4)}$$\n\nwe can substitute for $G(s)=\\frac{150}{s}$:\n\n$$\\frac{H(s)}{G(s)}=\\frac{(2s^3+11s^2+4s+12)}{(s^4+3s^3+7s^2+4)}$$\n\n$$\\frac{H(s)}{(\\frac{150}{s})}=\\frac{(2s^3+11s^2+4s+12)}{(s^4+3s^3+7s^2+4)}$$\n\n$$\\frac{H(s)}{(\\frac{150}{s})}=\\frac{(2s^3+11s^2+4s+12)}{(s^4+3s^3+7s^2+4)}$$\n\nand isolate on $H(s)$:\n\n$$H(s)=\\frac{(2s^3+11s^2+4s+12)}{(s^4+3s^3+7s^2+4)}\\frac{150}{s}$$\n\nsince we now have managed to make a function for the output we can now use the final value theorem:\n\n$$\\lim_{s\\rightarrow\\infty}{\\{sH(s)\\}} = \\lim_{t\n\\rightarrow\\infty}{\\{h(t)\\}}$$"},{"metadata":{"trusted":true},"cell_type":"code","source":"import sympy as sym\ns,t = sym.symbols(\"s,t\")\n\n\nnum = [2,11,4,12]\ndenum = [1,3,7,0,4]\nW=(sym.Poly(num,s)/sym.Poly(denum,s))\n\nG=150/s\n\ndisplay(W)\n\nH=W*G\ndisplay(H)\n\nVfv = (s*H).subs(s,0)\ndisplay(Vfv)","execution_count":1,"outputs":[{"output_type":"display_data","data":{"text/plain":"(2*s**3 + 11*s**2 + 4*s + 12)/(s**4 + 3*s**3 + 7*s**2 + 4)","text/latex":"$\\displaystyle \\frac{2 s^{3} + 11 s^{2} + 4 s + 12}{s^{4} + 3 s^{3} + 7 s^{2} + 4}$"},"metadata":{}},{"output_type":"display_data","data":{"text/plain":"150*(2*s**3 + 11*s**2 + 4*s + 12)/(s*(s**4 + 3*s**3 + 7*s**2 + 4))","text/latex":"$\\displaystyle \\frac{150 \\cdot \\left(2 s^{3} + 11 s^{2} + 4 s + 12\\right)}{s \\left(s^{4} + 3 s^{3} + 7 s^{2} + 4\\right)}$"},"metadata":{}},{"output_type":"display_data","data":{"text/plain":"450","text/latex":"$\\displaystyle 450$"},"metadata":{}}]},{"metadata":{},"cell_type":"markdown","source":"needs to verifyi can use this by finding the poles."},{"metadata":{"trusted":false},"cell_type":"code","source":"import sympy as sp\nimport control as ctrl\ns = sp.symbols(\"s\")\n\nnum = [2,11,4,12]\ndenum = [1,3,7,0,4]\nW = ctrl.TransferFunction(num,denum)\n\ndisplay(\"stable\" if all(sp.re(pole) < 0 for pole in W.poles()) else \"unstable\")","execution_count":1,"outputs":[{"output_type":"display_data","data":{"text/plain":"'unstable'"},"metadata":{}}]},{"metadata":{},"cell_type":"markdown","source":"it is unstable. so the final value theorem doesn't work. the value will most likely diverge towards infinity since the."},{"metadata":{},"cell_type":"markdown","source":"# Problem 3\n\nConsider the electrical circuit shown below with the output $i_L(t)$ and the input $i_G(t)$. The differential equations describing the reactive elements are $u_L(t) = L\\frac{di_L(t)}{dt} = L{i'}_L(t)$, $i_C(t) = C\\frac{du_C(t)}{dt} = C{u'}_C(t)$. The initial values are $i_L(0) = 0\\;[A]$"},{"metadata":{"trusted":false},"cell_type":"markdown","source":"## a)\n\nFind the differential eqiation of the circuit;"},{"metadata":{},"cell_type":"markdown","source":"$$i_G(t)=i_R+i_C+i_L$$\n\n$$i_R=\\frac{u_r}{R}$$\n\n$$i_C=C\\frac{du_C}{dt}$$\n\n$$u_L=L\\frac{di_L}{dt}$$\n\n$$i_G(t)=i_R+i_C+i_L$$\n\n$$i_G(t)-(i_R+i_C)=i_L$$\n\n$$i_G(t)-i_R-i_C=i_L$$\n\n$$i_L=i_G(t)-i_R-i_C$$\n\n$$i_L=i_G(t)-(\\frac{u_r}{R})-(C\\frac{du_C}{dt})$$\n\n$$ u_G = u_R = u_C = u_L + u_{R_L} = u $$\n\n$$i_L=i_G(t)-(\\frac{u}{R})-(C\\frac{du}{dt})$$"},{"metadata":{},"cell_type":"markdown","source":"$$i_G(t)=i_L+(\\frac{u}{R})+(C\\frac{du}{dt})$$\n\n$$i_G(t)=(L\\frac{di_L(t)}{dt})+(\\frac{u}{R})+(C\\frac{du}{dt})$$\n\n$$i_C=C\\frac{du_C}{dt}$$\n$$\\frac{1}{C}i_C=\\frac{du_C}{dt}$$\n$$\\frac{1}{C}\\int{i_C}=u_C$$\n\n$$i_G(t)=(L\\frac{di_L(t)}{dt})+(\\frac{u}{R})+(C\\frac{du}{dt})$$"},{"metadata":{},"cell_type":"markdown","source":""}],"metadata":{"kernelspec":{"name":"python3","display_name":"Python 3","language":"python"},"language_info":{"name":"python","version":"3.10.4","mimetype":"text/x-python","codemirror_mode":{"name":"ipython","version":3},"pygments_lexer":"ipython3","nbconvert_exporter":"python","file_extension":".py"}},"nbformat":4,"nbformat_minor":2}